DY/Trace/Invariant.lean
@@ -1,29 +1,28 @@
 module
 
 public import DY.Trace.Basic
+import all DY.Trace.Basic
 
 namespace DY
 
 public
-structure ProofEntryType (ExecEntryT: ExecEntryType) where
-  type: [ExecTraceTypes] → Type
-  erase: ∀ [ExecTraceTypes], type → ExecEntryT.type
+structure ProofEntryFun (ExecEntryT ProofEntryT: Type) where
+  erase: ProofEntryT → ExecEntryT
 
 public
-class ProofTraceTypes [ExecTraceTypes] where
-  proofEntries: ∀ id, ProofEntryType (ExecTraceTypes.entries id)
-
-public
-class abbrev TraceTypes := ExecTraceTypes, ProofTraceTypes
+class TraceTypes extends ExecTraceTypes where
+  proofEntries: Fin ExecTraceTypes.n → Type
+  funs: ∀ id, ProofEntryFun (ExecTraceTypes.entries id) (proofEntries id)
 
 public
 structure ProofTrace.Entry [TraceTypes] where
   id: Fin ExecTraceTypes.n
-  entry: (ProofTraceTypes.proofEntries id).type
+  entry: (TraceTypes.proofEntries id)
 
 public
 abbrev ProofTrace [TraceTypes] := Trace ProofTrace.Entry
 
+@[expose]
 public
 def ProofTrace.Entry.erase
   [TraceTypes]
@@ -31,7 +30,7 @@ def ProofTrace.Entry.erase
   : ExecTrace.Entry
 where
   id := entry.id
-  entry := (ProofTraceTypes.proofEntries entry.id).erase entry.entry
+  entry := (TraceTypes.funs entry.id).erase entry.entry
 
 public
 def Trace.erase
@@ -44,7 +43,9 @@ def Trace.erase
   | .snoc trBefore entry => .snoc trBefore.erase entry.erase
 
 public
-theorem Trace.erase_le [TraceTypes] (tr1 tr2: ProofTrace)
+theorem Trace.erase_le
+  [TraceTypes]
+  (tr1 tr2: ProofTrace)
   : tr1 ≤ tr2 →
     tr1.erase ≤ tr2.erase
 := by
@@ -56,35 +57,92 @@ theorem Trace.erase_le [TraceTypes] (tr1 tr2: ProofTrace)
 
 grind_pattern Trace.erase_le => tr1 ≤ tr2, tr1.erase
 
--- public
--- theorem Trace.erase_append
---   [TraceTypes]
---   (tr: ProofTrace) (entry: ProofTrace.Entry)
---   : (tr.append entry).erase = tr.erase.append entry.erase
--- := by
---   rfl
+public
+theorem Trace.erase_length
+  [TraceTypes]
+  (tr: ProofTrace)
+  : tr.erase.length = tr.length
+:= by
+  induction tr <;>
+  simp_all [Trace.length, Trace.erase]
 
--- TODO test coercion
-example [TraceTypes]: Coe ProofTrace ExecTrace where
-  coe tr := tr.erase
+public
+def Trace.erase_at
+  [TraceTypes]
+  (tr: ProofTrace)
+  (i: Nat) (h_i: i < tr.erase.length)
+  : tr.erase.at i h_i = (tr.at i (Trace.erase_length tr ▸ h_i)).erase
+:= by
+  induction tr <;>
+  simp only [Trace.at, Trace.erase]
+  · grind
+  split <;>
+  grind [Trace.erase_length]
+
+public
+class TraceTypes.Has [TraceTypes] {ExecEntryT: outParam Type} {ProofEntryT: Type} (func: outParam (ProofEntryFun ExecEntryT ProofEntryT)) extends ExecTraceTypes.Has ExecEntryT where
+  proofInj: ProofEntryT → ProofTrace.Entry
+  proofProj: ProofTrace.Entry → Option ProofEntryT
+  proof_inj_proj_eq: ∀ x y, (proofProj x = some y) = (x = proofInj y)
+  proofProj_none_eq_erase: ∀ x, ((proofProj x: Option ProofEntryT) = none) = ((proj x.erase: Option ExecEntryT) = none)
+  erase_commutes: ∀ entry, (proofInj entry).erase = inj (func.erase entry)
+
+public
+instance [TraceTypes] (id: Fin ExecTraceTypes.n): TraceTypes.Has (TraceTypes.funs id) where
+  proofInj entry := { id, entry }
+  proofProj entry :=
+    if h: entry.id = id then
+      some (h ▸ entry.entry)
+    else
+      none
+  proof_inj_proj_eq x y := by
+    cases x
+    grind
+  proofProj_none_eq_erase x := by
+    simp [ExecTraceTypes.Has.proj, ProofTrace.Entry.erase]
+  erase_commutes _ := rfl
+
+public
+instance [TraceTypes] {ExecEntryT ProofEntryT: Type} (func: ProofEntryFun ExecEntryT ProofEntryT) [TraceTypes.Has func]: IntoTraceEntry ProofEntryT ProofTrace.Entry where
+  make entry := TraceTypes.Has.proofInj entry
+
+public
+theorem Trace.append_erase
+  [TraceTypes]
+  {ExecEntryT ProofEntryT: Type}
+  {func: ProofEntryFun ExecEntryT ProofEntryT}
+  [TraceTypes.Has func]
+  (tr: ProofTrace) (entry: ProofEntryT)
+  : (tr.append entry).erase = tr.erase.append (func.erase entry)
+:= by
+  simp [Trace.append, Trace.erase, IntoTraceEntry.make, TraceTypes.Has.erase_commutes]
 
 -- Invariant
 
 public
-structure ProofTraceEntryInvariant
-  [TraceTypes]
-  {ExecEntryT: ExecEntryType}
-  (ProofEntryT: ProofEntryType ExecEntryT)
-where
-  invariant: ProofTrace → ProofEntryT.type → Prop
+structure TraceEntryInvariant [TraceTypes] {ExecEntryT ProofEntryT: Type} (func: ProofEntryFun ExecEntryT ProofEntryT) where
+  invariant: ProofTrace → ProofEntryT → Prop
 
 public
-class ProofTraceInvariants [TraceTypes] where
-  invariants: ∀ id, ProofTraceEntryInvariant (ProofTraceTypes.proofEntries id)
+class TraceInvariant extends TraceTypes where
+  invs: ∀ id, TraceEntryInvariant (TraceTypes.funs id)
+
+-- TODO test coercion
+example [TraceInvariant]: Coe ProofTrace ExecTrace where
+  coe tr := tr.erase
+
+public
+def ProofTrace.Entry.Invariant
+  [TraceInvariant]
+  (trBefore: ProofTrace)
+  (entry: ProofTrace.Entry)
+  : Prop
+:=
+  (TraceInvariant.invs entry.id).invariant trBefore entry.entry
 
 public
 def Trace.Invariant
-  [TraceTypes] [ProofTraceInvariants]
+  [TraceInvariant]
   (tr: ProofTrace)
   : Prop
 :=
@@ -92,6 +150,40 @@ def Trace.Invariant
   | .nil => True
   | .snoc trBefore entry =>
     trBefore.Invariant ∧
-    (ProofTraceInvariants.invariants entry.id).invariant trBefore entry.entry
+    entry.Invariant trBefore
+
+public
+class TraceInvariant.Has
+  [TraceInvariant]
+  {ExecEntryT: Type} {ProofEntryT: Type}
+  {func: ProofEntryFun ExecEntryT ProofEntryT}
+  (inv: outParam (TraceEntryInvariant func))
+  extends toTraceTypes: TraceTypes.Has func
+  where
+  inv_commutes: ∀ trBefore entry, (proofInj entry).Invariant trBefore = inv.invariant trBefore entry
+
+public
+theorem Trace.invariant_append
+  [TraceInvariant]
+  {ExecEntryT ProofEntryT: Type}
+  {func: ProofEntryFun ExecEntryT ProofEntryT}
+  {inv: TraceEntryInvariant func}
+  [TraceInvariant.Has inv]
+  (tr: ProofTrace) (entry: ProofEntryT)
+  : (tr.append entry).Invariant = (tr.Invariant ∧ inv.invariant tr entry)
+:= by
+  simp [Trace.Invariant, Trace.append, IntoTraceEntry.make, TraceInvariant.Has.inv_commutes]
+
+public
+theorem Trace.invariant_at
+  [TraceInvariant]
+  (tr: ProofTrace)
+  (i: Nat)
+  (h_i: i < tr.length)
+  : tr.Invariant →
+    (tr.at i h_i).Invariant (tr.prefix i)
+:= by
+  fun_induction Trace.at <;>
+  grind [Trace.Invariant, Trace.prefix, Trace.length]
 
 end DY
