DY/Actions/Network.lean
@@ -1,0 +1,98 @@
+module
+
+public import DY.Trace
+public import DY.Bytes
+public import DY.Trace.Manipulation
+import DY.Step.Init
+
+namespace DY
+
+namespace Network
+
+variable [BytesFunctor]
+
+public
+structure MsgSent where
+  msg: Bytes
+
+@[expose]
+public
+def ExecEntryT: Type :=
+  MsgSent
+
+public
+def attKnows [ExecTraceTypes]: ExecEntryAttackerKnowledge ExecEntryT where
+  attackerKnows _ entry msg := msg = entry.msg
+
+@[expose]
+public
+def ProofEntryT: Type := MsgSent
+
+public
+def ProofEntryFunc: ProofEntryFun ExecEntryT ProofEntryT where
+  erase x := x
+
+public
+def Invariant [TraceTypes] [BytesInvariants]: TraceEntryInvariant ProofEntryFunc where
+  invariant tr entry :=
+    entry.msg.Publishable tr
+
+-- TODO attacker knowledge theorem
+
+public
+def sendMessage [BytesFunctor] [ExecTraceTypes] [ExecTraceTypes.Has ExecEntryT] (msg: Bytes): Traceful Nat :=
+  do
+  let time ← getTimestamp
+  let entry: ExecEntryT := MsgSent.mk msg
+  appendEntry entry
+  return time
+
+@[instance]
+public
+theorem sendMessage.spec
+  [TraceInvariant]
+  [BytesInvariants] [BytesInvariantsProofs]
+  [TraceInvariant.Has Invariant]
+  (msg: Bytes)
+  : HoareTriple
+    (sendMessage msg)
+    (fun tr => msg.Publishable tr)
+    (fun _ _ => True)
+:= by
+  apply HoareTriple.mk
+  unfold sendMessage
+  dsimp only
+  step
+  step with ⟨ MsgSent.mk msg ⟩ by simp_all [ProofEntryFunc, Invariant]
+  step
+  trivial
+
+public
+def receiveMessage [BytesFunctor] [ExecTraceTypes] [ExecTraceTypes.Has ExecEntryT] (timestamp: Nat): Traceful Bytes :=
+  do
+  let msg: ExecEntryT ← getEntry timestamp
+  return msg.msg
+
+@[instance]
+public
+theorem receiveMessage.spec
+  [TraceInvariant]
+  [BytesInvariants] [BytesInvariantsProofs]
+  [TraceInvariant.Has Invariant]
+  (timestamp: Nat)
+  : HoareTriple
+    (receiveMessage timestamp)
+    (fun _ => True)
+    (fun msg tr => msg.Publishable tr)
+:= by
+  apply HoareTriple.mk
+  unfold receiveMessage
+  step
+  have: msg.msg.Publishable tr := by grind [Invariant, ProofEntryFunc]
+  rename_i h_msg; clear h_msg
+  step
+  grind
+
+end Network
+
+end DY
