DY/EquationalTheory/Hash.lean
@@ -167,7 +167,7 @@ end Invariants
 
 section AttackerKnowledgeTheorem
 
-variable [TraceTypes]
+variable [TraceInvariant]
 variable [BytesFunctor] [BytesInvariants]
 variable [BytesFunctor.Has SubF]
 variable [BytesInvariants.Has invariants]
