DY/Step/Trace.lean
@@ -1,3 +1,5 @@
+module
+
 import Lean
 
 -- We can't define and use trace classes in the same file
