DY/Trace.lean
@@ -1,5 +1,6 @@
 module
 
 public import DY.Trace.Basic
+public import DY.Trace.AttackerKnowledge
 public import DY.Trace.Invariant
 public import DY.Trace.Manipulation
