DY/Trace/AttackerKnowledge.lean
@@ -1,11 +1,15 @@
-import DY.Bytes.Basic
-import DY.Trace.Basic
+module
+
+public import DY.Bytes.Basic
+public import DY.Trace.Basic
 
 namespace DY
 
-structure ExecEntryAttackerKnowledge [BytesFunctor] [ExecTraceTypes] (ExecEntryT: ExecEntryType) where
-  attackerKnows: ExecTrace → ExecEntryT.type → Bytes → Prop
+public
+structure ExecEntryAttackerKnowledge [BytesFunctor] [ExecTraceTypes] (ExecEntryT: Type) where
+  attackerKnows: ExecTrace → ExecEntryT → Bytes → Prop
 
+public
 class ExecTraceAttackerKnowledge [BytesFunctor] [ExecTraceTypes] where
   attackerKnows: ∀ id, ExecEntryAttackerKnowledge (ExecTraceTypes.entries id)
 
